sketch more stuff

isabelle/Combined/Distinct_Elem_Alg_Nondet.thy
@@ -29,28 +29,46 @@ definition eager_state_inv :: "'a list \<Rightarrow> coin_matrix \<Rightarrow> '
   (state_chi state =
     nondet_alg_aux (state_k state) xs \<phi>)"
 
+lemma eager_step_1_inv:
+  assumes i:"i < length xs"
+  assumes inv: "eager_state_inv (take i xs) \<phi> state"
+  shows "
+    eager_state_inv (take (i+1) xs) \<phi>
+      (run_reader (eager_step_1 xs i state) \<phi>)"
+  unfolding eager_step_1_def
+  apply (auto simp add: run_reader_simps)
+  sorry
+
+lemma eager_step_2_inv:
+  assumes i:"i < length xs"
+  assumes inv: "eager_state_inv (take (i+1) xs) \<phi> state"
+  shows "
+    eager_state_inv (take (i+1) xs) \<phi>
+      (run_reader (eager_step_2 xs i state) \<phi>)"
+  unfolding eager_step_2_def
+  apply (auto simp add: run_reader_simps Let_def)
+  sorry
+
 lemma eager_step_inv:
   assumes i:"i < length xs"
   assumes inv: "eager_state_inv (take i xs) \<phi> state"
   shows "
     eager_state_inv (take (i+1) xs) \<phi>
       (run_reader (eager_step xs i state) \<phi>)"
-  sorry
+  by (metis eager_step_1_inv eager_step_2_inv eager_step_split i inv run_reader_simps(3))
 
 lemma eager_algorithm_inv:
   shows "eager_state_inv xs \<phi>
       (run_reader (eager_algorithm xs) \<phi>)"
-  unfolding eager_algorithm_def
-proof (induction xs)
+proof (induction xs rule:rev_induct)
   case Nil
   then show ?case
-    unfolding eager_state_inv_def nondet_alg_aux_def initial_state_def
-    by (auto simp add: run_reader_simps)
+    by (auto simp add: eager_algorithm_def run_reader_simps eager_state_inv_def initial_state_def nondet_alg_aux_def)
 next
-  case (Cons x xs)
+  case (snoc x xs)
   then show ?case
-    apply auto
-    sorry
+    apply (auto simp add: eager_algorithm_snoc)
+    by (metis (no_types, lifting) append_eq_conv_conj eager_step_inv length_append_singleton lessI list.sel(1) run_reader_simps(3) semiring_norm(174) take_hd_drop)
 qed
 
 lemma rel_pmf_eager_algorithm_nondet_alg_aux:
@@ -81,6 +99,59 @@ proof -
     by (metis simps(1) simps(2))
   finally show ?thesis .
 qed
+
+lemma filter_with_upto:
+  shows"
+  filter P [0..<n] =
+  filter (\<lambda>i. P i \<and> i < n) [0..<n]"
+  by (intro filter_cong) auto
+
+lemma find_last_eq:
+  assumes "x \<in> set xs"
+  shows "map_of (rev (zip xs [0..<length xs])) x = Some (find_last x xs)"
+  using assms
+proof (induction xs rule:rev_induct)
+  case Nil
+  then show ?case
+    by (auto simp add: find_last_def)
+next
+  case ih:(snoc x xs)
+  have *:"(filter
+             (\<lambda>i. (i < length xs \<longrightarrow>
+                    xs ! i = xs ! xb) \<and>
+                   (\<not> i < length xs \<longrightarrow>
+                    [x] ! (i - length xs) = xs ! xb))
+             [0..<length xs])
+    = filter (\<lambda>i. xs ! i = xs ! xb)
+             [0..<length xs]" for xb
+    apply (intro filter_cong)
+    by auto
+  show ?case
+    using ih
+    apply (auto simp add: nth_append
+       find_last_def Let_def filter_empty_conv *
+       split: if_splits)
+    using atLeastLessThan_iff by blast
+qed
+
+lemma nondet_alg_aux_eq_map_of:
+  shows "
+  nondet_alg_aux k xs \<phi> = (
+  let m = map_of (rev (zip xs [0..<length xs])) in
+  {y \<in> set xs.
+    (\<forall>k' < k. \<phi> (k', the (m y)))})"
+  using find_last_eq nondet_alg_aux_def by force
+
+definition nondet_alg :: "nat \<Rightarrow> ((nat \<times> 'a) \<Rightarrow> bool) \<Rightarrow> 'a set"
+  where "nondet_alg k \<phi> =
+  {y. (\<forall>k' < k. \<phi> (k', y))}"
+
+(* Removing the use of "find_last"? *)
+lemma nondet_alg_eq:
+  shows "
+    map_pmf (nondet_alg_aux K xs) (prod_pmf ({..<n}\<times>{..<n}) (\<lambda>_. coin_pmf)) =
+    map_pmf (nondet_alg K) (prod_pmf ({..<n}\<times> set xs) (\<lambda>_. coin_pmf))"
+  sorry
 
 end
 
